examples/xlrup_checker/xlrup_parsingScript.sml
@@ -5,6 +5,30 @@ open preamble miscTheory cnf_xorTheory xlrupTheory mlintTheory;
 
 val _ = new_theory "xlrup_parsing";
 
+val fromString_unsafe_def = Define`
+  fromString_unsafe str =
+    if strlen str = 0
+    then 0i
+    else if strsub str 0 = #"-"
+      then ~&fromChars_unsafe (strlen str - 1)
+                              (substring str 1 (strlen str - 1))
+      else &fromChars_unsafe (strlen str) str`;
+
+(* lowercase alphabet *)
+Definition is_lowercase_def:
+  is_lowercase c ⇔
+  #"a" ≤ c ∧ c ≤ #"z"
+End
+
+val tokenize_fast_def = Define`
+  tokenize_fast (s:mlstring) =
+  if strlen s = 0 then INL s
+  else if is_lowercase (strsub s 0) then INL s
+  else INR (fromString_unsafe s)`
+
+val toks_fast_def = Define`
+  toks_fast s = MAP tokenize_fast (tokens blanks s)`
+
 Definition parse_until_zero_def:
   (parse_until_zero [] acc = NONE) ∧
   (parse_until_zero (x::xs) acc =
@@ -32,57 +56,74 @@ Definition parse_until_zero_nn_def:
   )
 End
 
-Definition parse_rup_def:
-  (parse_rup (cid::rest) =
-  case cid of
-    INL _ => NONE
-  | INR n =>
-    if n ≥ 0 then
-      case parse_until_zero rest [] of
-        NONE => NONE
-      | SOME (c ,rest) =>
-        (case parse_until_zero_nn rest [] of
-          SOME (hints, []) =>
-          SOME (RUP (Num (ABS n)) c hints)
-        | _ => NONE)
-    else NONE) ∧
-  (parse_rup _ = NONE)
+(* Parses the following format:
+   (int list) 0 (num list) 0 *)
+Definition parse_rest_def:
+  parse_rest rest =
+  case parse_until_zero rest [] of
+    NONE => NONE
+  | SOME (c ,rest) =>
+    (case parse_until_zero_nn rest [] of
+      SOME (hints, []) => SOME (c,hints)
+    | _ => NONE)
 End
 
+(* Parses the following format:
+   num (int list) 0 (num list) 0 *)
+Definition parse_id_rest_def:
+  (parse_id_rest (id::rest) =
+  case id of INL _ => NONE
+  | INR n =>
+    if n ≥ 0 then
+      case parse_rest rest of NONE => NONE
+      | SOME (c,hints) => SOME(Num (ABS n), c, hints)
+    else NONE) ∧
+  (parse_id_rest _ = NONE)
+End
+
+(* Parses the following format:
+  d (num list) *)
 Definition parse_del_def:
-  (parse_del (cid::first::rest) =
-    case cid of INL i => NONE
-    | INR _ =>
-    (case parse_until_zero_nn rest [] of
-     SOME (ls, []) => SOME (Del ls)
-    | _ => NONE)) ∧
+  (parse_del (first::rest) =
+    if first = INL (strlit "d")
+    then
+      case parse_until_zero_nn rest [] of
+       SOME (ls, []) => SOME ls
+      | _ => NONE
+    else NONE) ∧
   (parse_del _ = NONE)
 End
 
-Definition parse_xdel_def:
-  (parse_xdel (cid::first::rest) =
-    if cid = INL (strlit "x")
-    then
-      (case parse_until_zero_nn rest [] of
-       SOME (ls, []) => SOME (XDel ls)
-      | _ => NONE)
-    else NONE) ∧
-  (parse_xdel _ = NONE)
-End
-
 Definition parse_xlrup_def:
-  parse_xlrup ls =
-  case parse_rup ls of SOME res => SOME res
-  | NONE =>
-  case parse_del ls of SOME res => SOME res
-  | NONE =>
-  case parse_xdel ls of SOME res => SOME res
-  | NONE => NONE
+  (parse_xlrup [] = NONE) ∧
+  (parse_xlrup (f::rest) =
+  case f of
+  | INR n =>
+    if n ≥ 0 then
+      case parse_del rest of
+        (* RUP *)
+        NONE =>
+        (case parse_rest rest of NONE => NONE
+        | SOME (c,hints) => SOME (RUP (Num (ABS n)) c hints))
+        (* Del *)
+      | SOME ls => SOME (Del ls)
+    else NONE
+  | INL c =>
+    if c = strlit"x"
+    then
+      case parse_del rest of
+        (* XAdd *)
+        NONE =>
+        (case parse_id_rest rest of NONE => NONE
+        | SOME (n,c,hints) => SOME (XAdd n c hints))
+        (* XDel *)
+      | SOME ls => SOME (XDel ls)
+    else NONE)
 End
 
 Theorem parse_xlrup_wf:
-  parse_xlrup ls = SOME xlrup ⇒
-  wf_xlrup xlrup
+  parse_xlrup ls = SOME line ⇒
+  wf_xlrup line
 Proof
   rw[parse_xlrup_def]>>
   gvs[AllCaseEqs()]>>
@@ -93,7 +134,7 @@ QED
 Definition parse_xlrups_def:
   (parse_xlrups [] = SOME []) ∧
   (parse_xlrups (l::ls) =
-    case parse_xlrup (MAP tokenize (tokens blanks l)) of
+    case parse_xlrup (toks_fast l) of
       NONE => NONE
     | SOME step =>
       (case parse_xlrups ls of
@@ -122,6 +163,7 @@ val xlrupsraw = ``[
   strlit"10 6 2 0 3 4 8 0";
   strlit"11 6 3 0 5 6 8 0";
   strlit"12 -6 4 0 1 5 7 3 0";
+  strlit"x 1234 -6 4 0 1 5 7 3 0";
   strlit"12 d 1 5 3 0";
   strlit"13 -6 5 0 2 6 7 4 0";
   strlit"13 d 2 6 4 0";
